Weidenbach_Book/IsaSAT_Setup.thy
@@ -631,7 +631,9 @@ definition twl_st_heur :: \<open>(twl_st_wl_heur \<times> nat twl_st_wl) set\<cl
     out_learned M D outl \<and>
     lcount = size (learned_clss_lf N) \<and>
     vdom_m (all_atms N (NE + UE))  W N \<subseteq> set vdom \<and>
-    set avdom \<subseteq> set vdom
+    set avdom \<subseteq> set vdom \<and>
+    isasat_input_bounded (all_atms N (NE + UE)) \<and>
+    isasat_input_nempty (all_atms N (NE + UE))
   }\<close>
 
 lemma twl_st_heur_state_simp:
@@ -671,7 +673,9 @@ where
     out_learned M D outl \<and>
     lcount = size (learned_clss_lf N) \<and>
     vdom_m (all_atms N (NE + UE)) W N \<subseteq> set vdom \<and>
-    set avdom \<subseteq> set vdom
+    set avdom \<subseteq> set vdom \<and>
+    isasat_input_bounded (all_atms N (NE + UE)) \<and>
+    isasat_input_nempty (all_atms N (NE + UE))
   }\<close>
 
 lemma twl_st_heur_twl_st_heur_conflict_ana:
@@ -704,7 +708,9 @@ definition twl_st_heur_bt :: \<open>(twl_st_wl_heur \<times> nat twl_st_wl) set\
     out_learned M None outl \<and>
     lcount = size (learned_clss_l N) \<and>
     vdom_m (all_atms N (NE + UE)) W N \<subseteq> set vdom \<and>
-    set avdom \<subseteq> set vdom
+    set avdom \<subseteq> set vdom \<and>
+    isasat_input_bounded (all_atms N (NE + UE)) \<and>
+    isasat_input_nempty (all_atms N (NE + UE))
   }\<close>
 
 
